remove my_tid from isim: finish CRIS.v Cancel.v

theories/simulations/isim/ISim.v
@@ -9,11 +9,10 @@ Section SIM.
   Context `{Σ : GRA}.
   Variable contextual: contextuality.
   Variable fl_src fl_tgt : alist (option string) (Any.t → itree hmodE Any.t).
-  Variable Ist : nat → alist key Any.t → alist key Any.t → iProp Σ.
-  Variable stid : nat.
+  Variable Ist : ist_type Σ.
 
-  Let _hsim := _hsim contextual fl_src fl_tgt Ist stid.
-  Let rel := ∀ Rs Rt, (nat → alist key Any.t * Rs → alist key Any.t * Rt → iProp Σ) → bool → bool → nat → alist key Any.t * itree hmodE Rs → alist key Any.t * itree hmodE Rt → iProp Σ.
+  Let _hsim := _hsim contextual fl_src fl_tgt Ist.
+  Let rel := ∀ Rs Rt, (retr_type Σ Rs Rt) → bool → bool → nat → alist key Any.t * itree hmodE Rs → alist key Any.t * itree hmodE Rt → iProp Σ.
 
   Variant iunlift (r : rel) Rs Rt RR ps pt nths sti_src sti_tgt res : Prop :=
   | unlift_intro (WF : ✓ res) (REL : Own res ⊢ |==> r Rs Rt RR ps pt nths sti_src sti_tgt).
@@ -21,7 +20,7 @@ Section SIM.
   Definition ibot : rel := λ _ _ _ _ _ _ _ _, False%I.
 
   Global Program Definition isim
-      r g {Rs Rt} (RR : nat → alist key Any.t * Rs → alist key Any.t * Rt → iProp Σ) ps pt
+      r g {Rs Rt} (RR : retr_type Σ Rs Rt) ps pt
       nths sti_src sti_tgt : iProp Σ :=
     UPred Σ (gpaco9 (_hsim) (cpn9 _hsim) (iunlift r) (iunlift g) _ _ RR ps pt nths sti_src sti_tgt) _.
   Next Obligation. guclo hsim_extendC_spec. econs; et. Defined.
@@ -648,7 +647,7 @@ Section SIM.
           (NODS : List.NoDup (List.map fst st_src0))
           (NODD : List.NoDup (List.map fst st_tgt0))
           (NTHS: nths <= nths0),
-        (Ist nths0 st_src0 st_tgt0) -∗ @isim r g Rs Rt RR true true nths0 (st_src0, k_src stid) (st_tgt0, k_tgt stid))
+        (Ist nths0 st_src0 st_tgt0) -∗ @isim r g Rs Rt RR true true nths0 (st_src0, k_src ()) (st_tgt0, k_tgt ()))
     ⊢ (isim r g RR ps pt nths (st_src, trigger (Yield tid) >>= k_src) (st_tgt, trigger (Yield tid) >>= k_tgt)).
   Proof using.
     split; intros x wfx Hx. uPred.unseal_once_in Hx. destruct Hx as [x1 [x2 [-> [Hx1 Hx2]]]].
@@ -831,13 +830,12 @@ Section Proph.
 
   Context (contextual: contextuality).
   Context (fl_s fl_t : alist (option string) (Any.t → itree hmodE Any.t)).
-  Context (Ist : nat → alist key Any.t → alist key Any.t → iProp Σ).
-  Context (stid: nat).
+  Context (Ist : ist_type Σ).
 
-  Local Notation isim := (isim contextual fl_s fl_t Ist stid).
+  Local Notation isim := (isim contextual fl_s fl_t Ist).
 
   Context (R_s R_t : Type).
-  Context (RR : nat → alist key Any.t * R_s → alist key Any.t * R_t → iProp Σ).
+  Context (RR : retr_type Σ R_s R_t).
   Context (ps pt : bool).
   Context (nths : nat).
   Context (st_s st_t : alist key Any.t).
@@ -931,13 +929,12 @@ End Proph.
 
 Definition isim_fsem `{Σ : GRA} fl_src fl_tgt Ist contextual IstS IstE : relation (Any.t -> itree hmodE Any.t) :=
   fun itr_src itr_tgt =>
-  ∀ arg stid nths st_src st_tgt
+  ∀ arg nths st_src st_tgt
     (IMON : Ist_monotone Ist)
     (NODS : List.NoDup (List.map fst st_src))
-    (NODD : List.NoDup (List.map fst st_tgt))
-    (TID: stid < nths),
+    (NODD : List.NoDup (List.map fst st_tgt)),
   IstS nths st_src st_tgt ⊢
-    @isim Σ contextual fl_src fl_tgt Ist stid ibot ibot Any.t Any.t (ist_with_eq IstE)
+    @isim Σ contextual fl_src fl_tgt Ist ibot ibot Any.t Any.t (ist_with_eq IstE)
       false false nths (st_src, itr_src arg) (st_tgt, itr_tgt arg).
 
 Module HSim. Section HSim.
@@ -947,7 +944,7 @@ Module HSim. Section HSim.
   Variable contextual: contextuality.
   Variable (ms_src ms_tgt : HMod.t).
   Variable init_cond : iProp Σ.
-  Variable Ist : nat -> alist key Any.t -> alist key Any.t -> iProp Σ.
+  Variable Ist : ist_type Σ.
 
   Let scopes_src := ms_src.(scopes).
   Let scopes_tgt := ms_tgt.(scopes).
