theories/simulations/isim/ITactics.v
@@ -24,24 +24,24 @@ Ltac _istep_l :=
   match goal with
   (******* isim ******)
   (** src **)
-  | [ |- environments.envs_entails _ (isim _ _ _ _ _ _ _ _ _ _ _ (_, tau;; _) _) ] =>
+  | [ |- environments.envs_entails _ (isim _ _ _ _ _ _ _ _ _ _ (_, tau;; _) _) ] =>
       iApply isim_tau_src
-  | [ |- environments.envs_entails _ (isim _ _ _ _ _ _ _ _ _ _ _ (_, Ret _ >>= _) _) ] =>
+  | [ |- environments.envs_entails _ (isim _ _ _ _ _ _ _ _ _ _ (_, Ret _ >>= _) _) ] =>
       rewrite bind_ret_l
-  | [ |- environments.envs_entails _ (isim _ _ _ _ _ _ _ _ _ _ _ (_, (SB.sandbox _ _ _ (trigger (SPut _ _))) >>= _) _) ] =>
+  | [ |- environments.envs_entails _ (isim _ _ _ _ _ _ _ _ _ _ (_, (SB.sandbox _ _ _ (trigger (SPut _ _))) >>= _) _) ] =>
       iApply isim_sput_src_sandbox; [s;eauto|]
-  | [ |- environments.envs_entails _ (isim _ _ _ _ _ _ _ _ _ _ _ (_, (SB.sandbox _ _ _ (trigger (SGet _))) >>= _) _) ] =>
+  | [ |- environments.envs_entails _ (isim _ _ _ _ _ _ _ _ _ _ (_, (SB.sandbox _ _ _ (trigger (SGet _))) >>= _) _) ] =>
       iApply isim_sget_src_sandbox; [s;eauto|]
-  | [ |- environments.envs_entails _ (isim _ _ _ _ _ _ _ _ _ _ _ (_, trigger (Take _) >>= _) _) ] =>
+  | [ |- environments.envs_entails _ (isim _ _ _ _ _ _ _ _ _ _ (_, trigger (Take _) >>= _) _) ] =>
       let name := fresh "q" in
       iApply isim_take_src; iIntros (name)
-  | [ |- environments.envs_entails _ (isim _ _ _ _ _ _ _ _ _ _ _  (_, trigger (Assume ?P) >>= _) _) ] =>
+  | [ |- environments.envs_entails _ (isim _ _ _ _ _ _ _ _ _ _  (_, trigger (Assume ?P) >>= _) _) ] =>
       unfold_precond_postcond P; iApply isim_assume_src; iIntrosFresh "ASM"
-  | [ |- environments.envs_entails _ (isim _ _ _ _ _ _ _ _ _ _ _ (_, unwrapU ?ox >>= _) _) ] =>
+  | [ |- environments.envs_entails _ (isim _ _ _ _ _ _ _ _ _ _ (_, unwrapU ?ox >>= _) _) ] =>
       let name := fresh "q" in
       iApply isim_unwrapU_src; iIntros (name) "%";
       match goal with [ H: ?x = Some _ |- _ ] => let G := fresh "G" in rename H into G; try rewrite -> G in * end
-  | [ |- environments.envs_entails _ (isim _ _ _ _ _ _ _ _ _ _ (_, assume _ >>= _) _) ] =>
+  | [ |- environments.envs_entails _ (isim _ _ _ _ _ _ _ _ _ (_, assume _ >>= _) _) ] =>
       let name := fresh "asm" in iApply isim_asm_src; iIntros (name)
   end.
 
@@ -62,24 +62,24 @@ Ltac _istep_r :=
   match goal with
   (******* isim ******)
   (** tgt **)
-  | [ |- environments.envs_entails _ (isim _ _ _ _ _ _ _ _ _ _ _ _ (_, Ret _ >>= _)) ] =>
+  | [ |- environments.envs_entails _ (isim _ _ _ _ _ _ _ _ _ _ _ (_, Ret _ >>= _)) ] =>
       rewrite bind_ret_l
-  | [ |- environments.envs_entails _ (isim _ _ _ _ _ _ _ _ _ _ _ _ (_, tau;; _)) ] =>
+  | [ |- environments.envs_entails _ (isim _ _ _ _ _ _ _ _ _ _ _ (_, tau;; _)) ] =>
       iApply isim_tau_tgt
-  | [ |- environments.envs_entails _ (isim _ _ _ _ _ _ _ _ _ _ _ _ (_, (SB.sandbox _ _ _ (trigger (SPut _ _))) >>= _)) ] =>
+  | [ |- environments.envs_entails _ (isim _ _ _ _ _ _ _ _ _ _ _ (_, (SB.sandbox _ _ _ (trigger (SPut _ _))) >>= _)) ] =>
       iApply isim_sput_tgt_sandbox; [s; eauto|]
-  | [ |- environments.envs_entails _ (isim _ _ _ _ _ _ _ _ _ _ _ _ (_, (SB.sandbox _ _ _ (trigger (SGet _))) >>= _)) ] =>
+  | [ |- environments.envs_entails _ (isim _ _ _ _ _ _ _ _ _ _ _ (_, (SB.sandbox _ _ _ (trigger (SGet _))) >>= _)) ] =>
       iApply isim_sget_tgt_sandbox; [s; eauto|]
-  | [ |- environments.envs_entails _ (isim _ _ _ _ _ _ _ _ _ _ _ _ (_, trigger (Choose _) >>= _)) ] =>
+  | [ |- environments.envs_entails _ (isim _ _ _ _ _ _ _ _ _ _ _ (_, trigger (Choose _) >>= _)) ] =>
       let name := fresh "q" in
       iApply isim_choose_tgt; iIntros (name)
-  | [ |- environments.envs_entails _ (isim _ _ _ _ _ _ _ _ _ _ _ _ (_, trigger (Guarantee ?P) >>= _)) ] =>
+  | [ |- environments.envs_entails _ (isim _ _ _ _ _ _ _ _ _ _ _ (_, trigger (Guarantee ?P) >>= _)) ] =>
       unfold_precond_postcond P; iApply isim_guarantee_tgt; iIntrosFresh "GRT"
-  | [ |- environments.envs_entails _ (isim _ _ _ _ _ _ _ _ _ _ _ _ (_, unwrapN ?ox >>= _)) ] =>
+  | [ |- environments.envs_entails _ (isim _ _ _ _ _ _ _ _ _ _ _ (_, unwrapN ?ox >>= _)) ] =>
       let name := fresh "q" in
       iApply isim_unwrapN_tgt; iIntros (name) "%";
       match goal with [ H: ?x = Some _ |- _ ] => let G := fresh "G" in rename H into G; try rewrite -> G in * end
-  | [ |- environments.envs_entails _ (isim _ _ _ _ _ _ _ _ _ _ _ _ (_, guarantee _ >>= _)) ] =>
+  | [ |- environments.envs_entails _ (isim _ _ _ _ _ _ _ _ _ _ _ (_, guarantee _ >>= _)) ] =>
       let name := fresh "grt" in iApply isim_guar_tgt; iIntros (name)
   end.
 
@@ -100,11 +100,11 @@ Ltac _istep :=
   match goal with
   (******* isim ******)
   (** both **)
-  | [ |- environments.envs_entails _ (isim _ _ _ _ _ _ _ _ _ _ _ (_, Ret _) (_, Ret _)) ] =>
+  | [ |- environments.envs_entails _ (isim _ _ _ _ _ _ _ _ _ _ (_, Ret _) (_, Ret _)) ] =>
       iApply isim_ret
-  | [ |- environments.envs_entails _ (isim _ _ _ _ _ _ _ _ _ _ _ (_, trigger (IO _ _) >>= _) (_, trigger (IO _ _) >>= _)) ] =>
+  | [ |- environments.envs_entails _ (isim _ _ _ _ _ _ _ _ _ _ (_, trigger (IO _ _) >>= _) (_, trigger (IO _ _) >>= _)) ] =>
       iApply isim_io; iIntros "%"
-  | [ |- environments.envs_entails _ (isim _ _ _ _ _ _ _ _ _ _ _ (_, trigger (AssumePrecise _) >>= _) (_, trigger (AssumePrecise _) >>= _)) ] =>
+  | [ |- environments.envs_entails _ (isim _ _ _ _ _ _ _ _ _ _ (_, trigger (AssumePrecise _) >>= _) (_, trigger (AssumePrecise _) >>= _)) ] =>
       iApply isim_assume_precise_both
   end.
 
@@ -113,15 +113,15 @@ Ltac istep :=
 
 Ltac _iforce_l :=
   match goal with
-  | [ |- environments.envs_entails _ (isim _ _ _ _ _ _ _ _ _ _ _ (_, trigger (Choose ?T) >>= _) _) ] =>
+  | [ |- environments.envs_entails _ (isim _ _ _ _ _ _ _ _ _ _ (_, trigger (Choose ?T) >>= _) _) ] =>
       iApply isim_choose_src
-  | [ |- environments.envs_entails _ (isim _ _ _ _ _ _ _ _ _ _ _ (_, trigger (Guarantee ?P) >>= _) _) ] =>
+  | [ |- environments.envs_entails _ (isim _ _ _ _ _ _ _ _ _ _ (_, trigger (Guarantee ?P) >>= _) _) ] =>
       unfold_precond_postcond P; iApply isim_guarantee_src
-  | [ |- environments.envs_entails _ (isim _ _ _ _ _ _ _ _ _ _ _ (_, trigger (AssumePrecise ?P) >>= _) _) ] =>
+  | [ |- environments.envs_entails _ (isim _ _ _ _ _ _ _ _ _ _ (_, trigger (AssumePrecise ?P) >>= _) _) ] =>
       iApply isim_assume_precise_src; iSplitL "";[|iIntrosFresh "ASM"]
-  | [ |- environments.envs_entails _ (isim _ _ _ _ _ _ _ _ _ _ _ (_, unwrapN _ >>= _) _) ] =>
+  | [ |- environments.envs_entails _ (isim _ _ _ _ _ _ _ _ _ _ (_, unwrapN _ >>= _) _) ] =>
       iApply isim_unwrapN_src; iExists _
-  | [ |- environments.envs_entails _ (isim _ _ _ _ _ _ _ _ _ _ _ (_, guarantee _ >>= _) _) ] =>
+  | [ |- environments.envs_entails _ (isim _ _ _ _ _ _ _ _ _ _ (_, guarantee _ >>= _) _) ] =>
       iApply isim_guar_src
   end
 .
@@ -140,17 +140,17 @@ Ltac iforces_l :=
 
 Ltac _iforce_r :=
   match goal with
-  | [ |- environments.envs_entails _ (isim _ _ _ _ _ _ _ _ _ _ _ _ (_, trigger (Take _) >>= _)) ] =>
+  | [ |- environments.envs_entails _ (isim _ _ _ _ _ _ _ _ _ _ _ (_, trigger (Take _) >>= _)) ] =>
       iApply isim_take_tgt
-  | [ |- environments.envs_entails _ (isim _ _ _ _ _ _ _ _ _ _ _ _ (_, trigger (Assume ?P) >>= _)) ] =>
+  | [ |- environments.envs_entails _ (isim _ _ _ _ _ _ _ _ _ _ _ (_, trigger (Assume ?P) >>= _)) ] =>
       unfold_precond_postcond P; iApply isim_assume_tgt
-  | [ |- environments.envs_entails _ (isim _ _ _ _ _ _ _ _ _ _ _ _ (_, trigger (AssumePrecise ?P) >>= _)) ] =>
+  | [ |- environments.envs_entails _ (isim _ _ _ _ _ _ _ _ _ _ _ (_, trigger (AssumePrecise ?P) >>= _)) ] =>
       unfold_precond_postcond P; iApply isim_assume_precise_tgt; [..|iIntrosFresh "PRECISE"]
-  | [ |- environments.envs_entails _ (isim _ _ _ _ _ _ _ _ _ _ _ _ (_, AssumeProph _ _ >>= _)) ] =>
+  | [ |- environments.envs_entails _ (isim _ _ _ _ _ _ _ _ _ _ _ (_, AssumeProph _ _ >>= _)) ] =>
       iApply isim_assume_proph_tgt
-  | [ |- environments.envs_entails _ (isim _ _ _ _ _ _ _ _ _ _ _ _ (_, assume _ >>= _)) ] =>
+  | [ |- environments.envs_entails _ (isim _ _ _ _ _ _ _ _ _ _ _ (_, assume _ >>= _)) ] =>
       iApply isim_asm_tgt
-  | [ |- environments.envs_entails _ (isim _ _ _ _ _ _ _ _ _ _ _ _ (_, unwrapU _ >>= _)) ] =>
+  | [ |- environments.envs_entails _ (isim _ _ _ _ _ _ _ _ _ _ _ (_, unwrapU _ >>= _)) ] =>
       iApply isim_unwrapU_tgt; iExists _
   end
 .
