theories/simulations/wsim/WTactics.v
@@ -4,13 +4,13 @@ Require Import WSim TacticsCommon TacticsInit.
 
 Ltac _wstep_l :=
   match goal with
-  | [ |- environments.envs_entails _ (wsim _ _ _ _ _ _ _ _ _ _ _ _ _ (_, tau;; _) _) ] =>
+  | [ |- environments.envs_entails _ (wsim _ _ _ _ _ _ _ _ _ _ _ _ (_, tau;; _) _) ] =>
       iApply wsim_tau_src
-  | [ |- environments.envs_entails _ (wsim _ _ _ _ _ _ _ _ _ _ _ _ _ (_, Ret _ >>= _) _) ] =>
+  | [ |- environments.envs_entails _ (wsim _ _ _ _ _ _ _ _ _ _ _ _ (_, Ret _ >>= _) _) ] =>
       rewrite bind_ret_l
-  | [ |- environments.envs_entails _ (wsim _ _ _ _ _ _ _ _ _ _ _ _ _ (_, trigger (Take _) >>= _) _) ] =>
+  | [ |- environments.envs_entails _ (wsim _ _ _ _ _ _ _ _ _ _ _ _ (_, trigger (Take _) >>= _) _) ] =>
       let name := fresh "q" in iApply wsim_take_src; iIntros (name)
-  | [ |- environments.envs_entails _ (wsim _ _ _ _ _ _ _ _ _ _ _ _ _ (_, trigger (Assume ?P) >>= _) _) ] =>
+  | [ |- environments.envs_entails _ (wsim _ _ _ _ _ _ _ _ _ _ _ _ (_, trigger (Assume ?P) >>= _) _) ] =>
       first [
         tcsearch constr:(WP P)
           ltac:(fun c =>
@@ -21,13 +21,13 @@ Ltac _wstep_l :=
         end
       | unfold_precond_postcond P; iApply wsim_assume_src; iIntrosFresh "ASM"
       ]
-  | [ |- environments.envs_entails _ (wsim _ _ _ _ _ _ _ _ _ _ _ _ _ (_, assume _ >>= _) _) ] =>
+  | [ |- environments.envs_entails _ (wsim _ _ _ _ _ _ _ _ _ _ _ _ (_, assume _ >>= _) _) ] =>
       let name := fresh "asm" in iApply wsim_asm_src; iIntros (name)
-  | [ |- environments.envs_entails _ (wsim _ _ _ _ _ _ _ _ _ _ _ _ _ (_, (SB.sandbox _ _ _ (trigger (SPut _ _))) >>= _) _) ] =>
+  | [ |- environments.envs_entails _ (wsim _ _ _ _ _ _ _ _ _ _ _ _ (_, (SB.sandbox _ _ _ (trigger (SPut _ _))) >>= _) _) ] =>
       iApply wsim_sput_src_sandbox; [s;eauto|]
-  | [ |- environments.envs_entails _ (wsim _ _ _ _ _ _ _ _ _ _ _ _ _ (_, (SB.sandbox _ _ _ (trigger (SGet _))) >>= _) _) ] =>
+  | [ |- environments.envs_entails _ (wsim _ _ _ _ _ _ _ _ _ _ _ _ (_, (SB.sandbox _ _ _ (trigger (SGet _))) >>= _) _) ] =>
       iApply wsim_sget_src_sandbox; [s;eauto|]
-  | [ |- environments.envs_entails _ (wsim _ _ _ _ _ _ _ _ _ _ _ _ _ (_, unwrapU ?ox >>= _) _) ] =>
+  | [ |- environments.envs_entails _ (wsim _ _ _ _ _ _ _ _ _ _ _ _ (_, unwrapU ?ox >>= _) _) ] =>
       let name := fresh "q" in
       iApply wsim_unwrapU_src; iIntros (name) "%";
       match goal with [ H: ?x = Some _ |- _ ] => let G := fresh "G" in rename H into G; try rewrite -> G in * end
@@ -50,13 +50,13 @@ Ltac _wstep_r :=
   match goal with
   (******* isim ******)
   (** tgt **)
-  | [ |- environments.envs_entails _ (wsim _ _ _ _ _ _ _ _ _ _ _ _ _ _ (_, tau;; _)) ] =>
+  | [ |- environments.envs_entails _ (wsim _ _ _ _ _ _ _ _ _ _ _ _ _ (_, tau;; _)) ] =>
       iApply wsim_tau_tgt
-  | [ |- environments.envs_entails _ (wsim _ _ _ _ _ _ _ _ _ _ _ _ _ _ (_, Ret _ >>= _) ) ] =>
+  | [ |- environments.envs_entails _ (wsim _ _ _ _ _ _ _ _ _ _ _ _ _ (_, Ret _ >>= _) ) ] =>
       rewrite bind_ret_l
-  | [ |- environments.envs_entails _ (wsim _ _ _ _ _ _ _ _ _ _ _ _ _ _ (_, trigger (Choose _) >>= _) ) ] =>
+  | [ |- environments.envs_entails _ (wsim _ _ _ _ _ _ _ _ _ _ _ _ _ (_, trigger (Choose _) >>= _) ) ] =>
       let name := fresh "q" in iApply wsim_choose_tgt; iIntros (name)
-  | [ |- environments.envs_entails _ (wsim _ _ _ _ _ _ _ _ _ _ _ _ _ _ (_, trigger (Guarantee ?P) >>= _) ) ] =>
+  | [ |- environments.envs_entails _ (wsim _ _ _ _ _ _ _ _ _ _ _ _ _ (_, trigger (Guarantee ?P) >>= _) ) ] =>
       first [
         tcsearch constr:(WP P)
           ltac:(fun c =>
@@ -65,17 +65,17 @@ Ltac _wstep_r :=
         | [ |- environments.envs_entails _ (?P' -∗ _)] =>
           unfold_precond_postcond P'; iIntrosFresh "GRT";
           match goal with
-          | |- environments.envs_entails _ (wsim _ _ _ (Some (?E ∖ ?E' ∪ ?E', ?E ∖ ?E' ∪ ?E')) _ _ _ _ _ _ _ _ _ _) =>
+          | |- environments.envs_entails _ (wsim _ _ (Some (?E ∖ ?E' ∪ ?E', ?E ∖ ?E' ∪ ?E')) _ _ _ _ _ _ _ _ _ _) =>
             try (replace (E ∖ E' ∪ E') with E by set_solver)
           end
         end
       | unfold_precond_postcond P; iApply wsim_guarantee_tgt; iIntrosFresh "GRT"
       ]
-  | [ |- environments.envs_entails _ (wsim _ _ _ _ _ _ _ _ _ _ _ _ _ _ (_, guarantee _ >>= _)) ] =>
+  | [ |- environments.envs_entails _ (wsim _ _ _ _ _ _ _ _ _ _ _ _ _ (_, guarantee _ >>= _)) ] =>
       let name := fresh "grt" in iApply wsim_guar_tgt; iIntros (name)
-  | [ |- environments.envs_entails _ (wsim _ _ _ _ _ _ _ _ _ _ _ _ _ _ (_, (SB.sandbox _ _ _ (trigger (SPut _ _))) >>= _)) ] =>
+  | [ |- environments.envs_entails _ (wsim _ _ _ _ _ _ _ _ _ _ _ _ _ (_, (SB.sandbox _ _ _ (trigger (SPut _ _))) >>= _)) ] =>
       iApply wsim_sput_tgt_sandbox; [s; eauto|]
-  | [ |- environments.envs_entails _ (wsim _ _ _ _ _ _ _ _ _ _ _ _ _ _ (_, (SB.sandbox _ _ _ (trigger (SGet _))) >>= _)) ] =>
+  | [ |- environments.envs_entails _ (wsim _ _ _ _ _ _ _ _ _ _ _ _ _ (_, (SB.sandbox _ _ _ (trigger (SGet _))) >>= _)) ] =>
       iApply wsim_sget_tgt_sandbox; [s; eauto|]
   end.
 
@@ -94,11 +94,11 @@ Ltac wsteps_r :=
 
 Ltac _wstep :=
   match goal with
-  | [ |- environments.envs_entails _ (wsim _ _ _ _ _ _ _ _ _ _ _ _ _ (_, Ret _) (_, Ret _))] =>
+  | [ |- environments.envs_entails _ (wsim _ _ _ _ _ _ _ _ _ _ _ _ (_, Ret _) (_, Ret _))] =>
       iApply wsim_ret
-  | [ |- environments.envs_entails _ (wsim _ _ _ _ _ _ _ _ _ _ _ _ _ (_, trigger (IO _ _) >>= _) (_, trigger (IO _ _) >>= _))] =>
+  | [ |- environments.envs_entails _ (wsim _ _ _ _ _ _ _ _ _ _ _ _ (_, trigger (IO _ _) >>= _) (_, trigger (IO _ _) >>= _))] =>
       iApply wsim_io; iIntros "%"
-  | [ |- environments.envs_entails _ (wsim _ _ _ _ _ _ _ _ _ _ _ _ _ (_, trigger (AssumePrecise _) >>= _) (_, trigger (AssumePrecise _) >>= _))] =>
+  | [ |- environments.envs_entails _ (wsim _ _ _ _ _ _ _ _ _ _ _ _ (_, trigger (AssumePrecise _) >>= _) (_, trigger (AssumePrecise _) >>= _))] =>
       iApply wsim_assume_precise_both
   end.
 
@@ -107,9 +107,9 @@ Ltac wstep :=
 
 Ltac _wforce_l :=
   match goal with
-  | [ |- environments.envs_entails _ (wsim _ _ _ _ _ _ _ _ _ _ _ _ _ (_, trigger (Choose ?T) >>= _) _) ] =>
+  | [ |- environments.envs_entails _ (wsim _ _ _ _ _ _ _ _ _ _ _ _ (_, trigger (Choose ?T) >>= _) _) ] =>
       iApply wsim_choose_src
-  | [ |- environments.envs_entails _ (wsim _ _ _ _ (Some (?Ew, ?E)) _ _ _ _ _ _ _ _ (_, trigger (Guarantee ?P) >>= _) _) ] =>
+  | [ |- environments.envs_entails _ (wsim _ _ _ (Some (?Ew, ?E)) _ _ _ _ _ _ _ _ (_, trigger (Guarantee ?P) >>= _) _) ] =>
       first [
         tcsearch constr:(WP P)
           ltac:(fun c =>
@@ -120,13 +120,13 @@ Ltac _wforce_l :=
         end
       | unfold_precond_postcond P; iApply wsim_guarantee_src
       ]
-  | [ |- environments.envs_entails _ (wsim _ _ _ _ None _ _ _ _ _ _ _ _ (_, trigger (Guarantee ?P) >>= _) _) ] =>
+  | [ |- environments.envs_entails _ (wsim _ _ _ None _ _ _ _ _ _ _ _ (_, trigger (Guarantee ?P) >>= _) _) ] =>
       unfold_precond_postcond P; iApply wsim_guarantee_src
-  | [ |- environments.envs_entails _ (wsim _ _ _ _ _ _ _ _ _ _ _ _ _ (_, trigger (AssumePrecise _) >>= _) _) ] =>
+  | [ |- environments.envs_entails _ (wsim _ _ _ _ _ _ _ _ _ _ _ _ (_, trigger (AssumePrecise _) >>= _) _) ] =>
       iApply wsim_assume_precise_src; iSplit; [|iIntrosFresh "ASM"]
-  | [ |- environments.envs_entails _ (wsim _ _ _ _ _ _ _ _ _ _ _ _ _ (_, unwrapN _ >>= _) _) ] =>
+  | [ |- environments.envs_entails _ (wsim _ _ _ _ _ _ _ _ _ _ _ _ (_, unwrapN _ >>= _) _) ] =>
       iApply wsim_unwrapN_src
-  | [ |- environments.envs_entails _ (wsim _ _ _ _ _ _ _ _ _ _ _ _ _ (_, guarantee _ >>= _) _) ] =>
+  | [ |- environments.envs_entails _ (wsim _ _ _ _ _ _ _ _ _ _ _ _ (_, guarantee _ >>= _) _) ] =>
       iApply wsim_guar_src
   end.
 
@@ -144,9 +144,9 @@ Ltac wforces_l :=
 
 Ltac _wforce_r :=
   match goal with
-  | [ |- environments.envs_entails _ (wsim _ _ _ _ _ _ _ _ _ _ _ _ _ _ (_, trigger (Take _) >>= _)) ] =>
+  | [ |- environments.envs_entails _ (wsim _ _ _ _ _ _ _ _ _ _ _ _ _ (_, trigger (Take _) >>= _)) ] =>
       iApply wsim_take_tgt
-  | [ |- environments.envs_entails _ (wsim _ _ _ _ _ _ _ _ _ _ _ _ _ _ (_, trigger (Assume ?P) >>= _)) ] =>
+  | [ |- environments.envs_entails _ (wsim _ _ _ _ _ _ _ _ _ _ _ _ _ (_, trigger (Assume ?P) >>= _)) ] =>
       first [
         tcsearch constr:(WP P)
           ltac:(fun c =>
@@ -158,7 +158,7 @@ Ltac _wforce_r :=
         end
       | unfold_precond_postcond P; iApply wsim_assume_tgt
       ]
-  | [ |- environments.envs_entails _ (wsim _ _ _ _ _ _ _ _ _ _ _ _ _ _ (_, trigger (AssumePrecise ?P) >>= _)) ] =>
+  | [ |- environments.envs_entails _ (wsim _ _ _ _ _ _ _ _ _ _ _ _ _ (_, trigger (AssumePrecise ?P) >>= _)) ] =>
       first [
         tcsearch constr:(WP P)
           ltac:(fun c =>
@@ -169,9 +169,9 @@ Ltac _wforce_r :=
         end
       | unfold_precond_postcond P; iApply wsim_assume_precise_tgt; iIntrosFresh "PRECISE"
       ]
-  | [ |- environments.envs_entails _ (wsim _ _ _ _ _ _ _ _ _ _ _ _ _ _ (_, AssumeProph _ _ >>= _)) ] =>
+  | [ |- environments.envs_entails _ (wsim _ _ _ _ _ _ _ _ _ _ _ _ _ (_, AssumeProph _ _ >>= _)) ] =>
       iApply wsim_assume_proph_tgt
-  | [ |- environments.envs_entails _ (wsim _ _ _ _ _ _ _ _ _ _ _ _ _ _ (_, assume _ >>= _)) ] =>
+  | [ |- environments.envs_entails _ (wsim _ _ _ _ _ _ _ _ _ _ _ _ _ (_, assume _ >>= _)) ] =>
       iApply wsim_asm_tgt
   end
 .
